Lampe/Lampe/Tactic/SL.lean
@@ -1,119 +1,19 @@
 import Lampe.SeparationLogic.State
 import Lampe.SeparationLogic.SLP
 import Lampe.Tactic.SLNorm
+import Lampe.Tactic.SL.Term
 import Lampe.Syntax
 
 import Lean.Meta.Tactic.Simp.Main
 
 open Lampe
 
+open Lampe.SL
+
 open Lean Elab.Tactic Parser.Tactic Lean.Meta Qq
 
 initialize
   Lean.registerTraceClass `Lampe.SL
-
-inductive SLTerm where
-| top : SLTerm
-| star : Expr → SLTerm → SLTerm → SLTerm
-| lift : Expr → SLTerm
-| singleton : Expr → Expr → SLTerm
-| lmbSingleton : Expr → Expr → SLTerm
-| mvar : Expr → SLTerm
-| all : Expr → SLTerm
-| exi : Expr → SLTerm
-| wand : SLTerm → SLTerm → SLTerm
-| unrecognized : Expr → SLTerm
-
-def SLTerm.toString : SLTerm → String
-| top => "⊤"
-| wand a b => s!"{a.toString} -⋆ {b.toString}"
-| exi e => s!"∃∃ {e}"
-| all e => s!"∀∀ {e}"
-| star _ a b => s!"({a.toString} ⋆ {b.toString})"
-| lift e => s!"⟦{e.dbgToString}⟧"
-| singleton e₁ _ => s!"[{e₁.dbgToString} ↦ _]"
-| lmbSingleton e₁ _ => s!"[λ {e₁.dbgToString} ↦ _]"
-| mvar e => s!"MV{e.dbgToString}"
-| unrecognized e => s!"<unrecognized: {e.dbgToString}>"
-
-def SLTerm.printShape : SLTerm → String
-| SLTerm.top => "⊤"
-| wand a b => s!"({a.printShape} -⋆ {b.printShape})"
-| exi _ => s!"(∃∃)"
-| all _ => s!"(∀∀)"
-| star _ a b => s!"({a.printShape} ⋆ {b.printShape})"
-| lift _ => s!"⟦⟧"
-| singleton _ _ => s!"[_ ↦ _]"
-| lmbSingleton _ _ => s!"[λ _ ↦ _]"
-| mvar _ => s!"MV"
-| unrecognized _ => s!"<unrecognized>"
-
-
-def SLTerm.isMVar : SLTerm → Bool
-| SLTerm.mvar _ => true
-| _ => false
-
-def SLTerm.isTop : SLTerm → Bool
-| SLTerm.top => true
-| _ => false
-
-def SLTerm.isForAll : SLTerm → Bool
-| SLTerm.all _ => true
-| _ => false
-
-instance : ToString SLTerm := ⟨SLTerm.toString⟩
-
-instance : Inhabited SLTerm := ⟨SLTerm.top⟩
-
-partial def parseSLExpr (e: Expr): TacticM SLTerm := do
-  if e.isAppOf ``SLP.star then
-    let args := e.getAppArgs
-    let fst ← parseSLExpr (←liftOption args[2]?)
-    let snd ← parseSLExpr (←liftOption args[3]?)
-    return SLTerm.star e fst snd
-  if e.isAppOf ``State.valSingleton then
-    let args := e.getAppArgs
-    let fst ← liftOption args[1]?
-    let snd ← liftOption args[2]?
-    return SLTerm.singleton fst snd
-  else if e.isAppOf ``State.lmbSingleton then
-    let args := e.getAppArgs
-    let fst ← liftOption args[1]?
-    let snd ← liftOption args[2]?
-    return SLTerm.lmbSingleton fst snd
-  else if e.isAppOf ``SLP.top then
-    return SLTerm.top
-  else if e.isAppOf ``SLP.lift then
-    let args := e.getAppArgs
-    return SLTerm.lift (←liftOption args[2]?)
-  else if e.getAppFn.isMVar then
-    return SLTerm.mvar e
-  else if e.isAppOf ``SLP.forall' then
-    let args := e.getAppArgs
-    return SLTerm.all (←liftOption args[3]?)
-  else if e.isAppOf ``SLP.exists' then
-    let args := e.getAppArgs
-    return SLTerm.exi (←liftOption args[3]?)
-  else if e.isAppOf ``SLP.wand then
-    let args := e.getAppArgs
-    let lhs ← parseSLExpr (←liftOption args[2]?)
-    let rhs ← parseSLExpr (←liftOption args[3]?)
-    return SLTerm.wand lhs rhs
-  else pure $ .unrecognized e
-
-partial def parseEntailment (e: Expr): TacticM (SLTerm × SLTerm) := do
-  if e.isAppOf ``SLP.entails then
-    let args := e.getAppArgs
-    let pre ← parseSLExpr (←liftOption args[2]?)
-    let post ← parseSLExpr (←liftOption args[3]?)
-    return (pre, post)
-  else throwError "not an entailment {e}"
-
-partial def solvesSingleton (lhs : SLTerm) (rhsV : Expr): TacticM Bool :=
-  match lhs with
-  | SLTerm.singleton v _ => pure $ v == rhsV
-  | SLTerm.exi (Lean.Expr.lam _ _ body _) => do solvesSingleton (←parseSLExpr body) rhsV
-  | _ => pure false
 
 namespace Internal
 
@@ -124,6 +24,10 @@ theorem singleton_congr_star_mv {p} {r} {v₁ v₂ : AnyValue p}  (heq: v₁ = v
 
 theorem lmbSingleton_congr_star_mv {argTps outTp p} (r : FuncRef argTps outTp) (f : HList (Tp.denote p) argTps → Expr (Tp.denote p) outTp):
     ([λr ↦ f] ⊢ [λr ↦ f] ⋆ ⟦⟧) := by
+  simp
+  apply SLP.entails_self
+
+theorem entails_self_true {p} {R : SLP (State p)} : R ⊢ R ⋆ ⟦⟧ := by
   simp
   apply SLP.entails_self
 
@@ -235,16 +139,22 @@ theorem solve_pure_ent_pure [LawfulHeap α] {P Q : Prop} :
   unfold SLP.entails
   simp only [and_imp, forall_eq_apply_imp_iff, and_true, imp_self]
 
+theorem ent_congr {p} {P P' Q Q' : SLP (State p)} (h₁ : P = P') (h₂ : Q = Q') : (P' ⊢ Q') → (P ⊢ Q) := by
+  cases h₁
+  cases h₂
+  exact id
+
 end Internal
 
 structure SLGoals where
+  entailments : List MVarId
   props : List MVarId
   implicits : List MVarId
 
-def SLGoals.flatten (g : SLGoals): List MVarId := g.props ++ g.implicits
+def SLGoals.flatten (g : SLGoals): List MVarId := g.entailments ++ g.props ++ g.implicits
 
 instance : Append SLGoals where
-  append g₁ g₂ := { props := g₁.props ++ g₂.props, implicits := g₁.implicits ++ g₂.implicits }
+  append g₁ g₂ := { entailments := g₁.entailments ++ g₂.entailments, props := g₁.props ++ g₂.props, implicits := g₁.implicits ++ g₂.implicits }
 
 def Lean.MVarId.apply' (m: MVarId) (e: Expr): TacticM (List MVarId) := do
   trace[Lampe.SL] "Applying {e}"
@@ -255,57 +165,57 @@ Solves goals of the form `P ⊢ [r ↦ v] ⋆ ?_`, trying to copy as much eviden
 -/
 partial def solveSingletonStarMV (goal : MVarId) (lhs : SLTerm) (rhs : Expr): TacticM SLGoals := do
   match lhs with
-  | SLTerm.singleton v _ =>
+  | SLTerm.singleton _ v _ =>
     if v == rhs then
       let heq :: impl ← goal.apply' (←mkConstWithFreshMVarLevels ``Internal.singleton_congr_star_mv) | throwError "unexpect goals in singleton_congr_star_mv"
       let heq ← try heq.refl; pure []
         catch _ => pure [heq]
-      pure $ SLGoals.mk heq impl
+      pure $ SLGoals.mk [] heq impl
     else throwError "final singleton is not equal"
-  | SLTerm.lmbSingleton v _ =>
-    if (←isDefEq v rhs) then
+  | SLTerm.lmbSingleton _ v _ =>
+    if (← goal.withContext $ isDefEq v rhs) then
       let impl ← goal.apply' (←mkConstWithFreshMVarLevels ``Internal.lmbSingleton_congr_star_mv)
-      pure $ SLGoals.mk [] impl
+      pure $ SLGoals.mk [] [] impl
     else throwError "final lmb singleton is not equal"
-  | SLTerm.exi _ =>
+  | SLTerm.exi _ _ =>
     if (←solvesSingleton lhs rhs) then
       let heq :: impl ← goal.apply' (←mkConstWithFreshMVarLevels ``Internal.exists_singleton_congr_mv) | throwError "unexpect goals in exists_singleton_congr_mv"
       let heq ← try (←heq.intro1).2.refl; pure []
         catch _ => pure [heq]
-      pure $ SLGoals.mk heq impl
+      pure $ SLGoals.mk [] heq impl
     else
       throwError "existential cannot solve the singleton"
   | SLTerm.star _ l r =>
     match l with
-    | SLTerm.singleton v _ => do
+    | SLTerm.singleton _ v _ => do
       if v == rhs then
         let heq :: impl ← goal.apply' (←mkConstWithFreshMVarLevels ``Internal.singleton_congr_star) | throwError "unexpect goals in singleton_congr_star"
         let heq ← try heq.refl; pure []
           catch _ => pure [heq]
-        pure $ SLGoals.mk heq impl
+        pure $ SLGoals.mk [] heq impl
       else
         let hent :: impl ← goal.apply' (←mkConstWithFreshMVarLevels ``Internal.skip_impure_evidence) | throwError "unexpect goals in skip_impure_evidence"
         let goals ← solveSingletonStarMV hent r rhs
-        pure $ goals ++ SLGoals.mk [] impl
+        pure $ goals ++ SLGoals.mk [] [] impl
     | SLTerm.lift _ =>
       let hEnt :: impl ← goal.apply' (←mkConstWithFreshMVarLevels ``Internal.skip_pure_evidence) | throwError "unexpect goals in skip_pure_evidence"
       let (_, hEnt) ← hEnt.intro1
       let goals ← solveSingletonStarMV hEnt r rhs
-      pure $ goals ++ SLGoals.mk [] impl
-    | SLTerm.exi _ =>
+      pure $ goals ++ SLGoals.mk [] [] impl
+    | SLTerm.exi _ _ =>
       if (←solvesSingleton l rhs) then
         let hent :: impl ← goal.apply' (←mkConstWithFreshMVarLevels ``Internal.exists_singleton_congr_star) | throwError "unexpect goals in exists_singleton_congr_star"
         let hent ← try (←hent.intro1).2.refl; pure []
           catch _ => pure [hent]
-        pure $ SLGoals.mk hent impl
+        pure $ SLGoals.mk [] hent impl
       else
         let hEnt :: impl ← goal.apply' (←mkConstWithFreshMVarLevels ``Internal.skip_impure_evidence) | throwError "unexpect goals in skip_impure_evidence"
         let goals ← solveSingletonStarMV hEnt r rhs
-        pure $ goals ++ SLGoals.mk [] impl
+        pure $ goals ++ SLGoals.mk [] [] impl
     | _ =>
       let hEnt :: impl ← goal.apply' (←mkConstWithFreshMVarLevels ``Internal.skip_impure_evidence) | throwError "unexpect goals in skip_impure_evidence"
       let goals ← solveSingletonStarMV hEnt r rhs
-      pure $ goals ++ SLGoals.mk [] impl
+      pure $ goals ++ SLGoals.mk [] [] impl
   | _ => throwError "unrecognized shape in solveSingletonStarMV"
 
 
@@ -317,23 +227,23 @@ partial def solvePureStarMV (goal : MVarId) (lhs : SLTerm): TacticM SLGoals := w
   | .lift _ =>
     let g :: impls ← goal.apply' (←mkConstWithFreshMVarLevels ``Internal.solve_pure_ent_pure_star_mv) | throwError "unexpected goals in solve_pure_ent_pure_star_mv"
     let (_, g) ← g.intro1
-    pure $ SLGoals.mk [g] impls
+    pure $ SLGoals.mk [] [g] impls
   | .star _ l r => do
     match l with
     | .lift _ =>
       let hEnt :: impl ← goal.apply' (←mkConstWithFreshMVarLevels ``Internal.skip_pure_evidence) | throwError "unexpect goals in skip_pure_evidence"
       let (_, hEnt) ← hEnt.intro1
       let goals ← solvePureStarMV hEnt r
-      pure $ goals ++ SLGoals.mk [] impl
+      pure $ goals ++ SLGoals.mk [] [] impl
     | _ =>
       let hEnt :: impl ← goal.apply' (←mkConstWithFreshMVarLevels ``Internal.skip_impure_evidence) | throwError "unexpect goals in skip_impure_evidence"
       let goals ← solvePureStarMV hEnt r
-      pure $ goals ++ SLGoals.mk [] impl
-  | .singleton _ _
-  | .lmbSingleton _ _
-  | .exi _ =>
+      pure $ goals ++ SLGoals.mk [] [] impl
+  | .singleton _ _ _
+  | .lmbSingleton _ _ _
+  | .exi _ _ =>
       let final :: impl ← goal.apply' (←mkConstWithFreshMVarLevels ``Internal.skip_evidence_and_solve_pure) | throwError "unexpected goals in skip_evidence_and_solve_pure"
-      pure $ SLGoals.mk [final] impl
+      pure $ SLGoals.mk [] [final] impl
   | _ => throwError "Unrecognized shape in solvePureStarMV"
 
 /--
@@ -343,14 +253,42 @@ def solvePureEntailMV (goal : MVarId) (preExpr : Lean.Expr) : TacticM SLGoals :=
   let g :: impls ← goal.apply' (←mkConstWithFreshMVarLevels ``Internal.solve_pure_ent_pure) | throwError "unexpected goals in solve_pure_ent_pure"
   let gs ← evalTacticAt (←`(tactic|try tauto)) g
   if gs.isEmpty then
-    return SLGoals.mk [] impls
+    return SLGoals.mk [] [] impls
   else
     -- If we are left in a `True → P` goal state then replace this with `P`
-    if preExpr.isAppOf ``True then
+    if preExpr.isAppOf' ``True then
       let mut (trueVar, g) ← g.intro1
       g ← g.clear trueVar
-      return SLGoals.mk [g] impls
-    return SLGoals.mk [g] impls
+      return SLGoals.mk [] [g] impls
+    return SLGoals.mk [] [g] impls
+
+def solveExactStarMV (goal: MVarId) (lhs : SLTerm) (rhs : Expr): TacticM SLGoals := withTraceNode `Lampe.SL (fun e => return f!"solveExactStarMV {Lean.exceptEmoji e}") do
+  match lhs with
+  | SLTerm.unrecognized expr =>
+    if (←isDefEq expr rhs) then
+      let impl ← goal.apply' (←mkConstWithFreshMVarLevels ``Internal.entails_self_true)
+      pure $ SLGoals.mk [] [] impl
+    else throwError "final unrecognized is not equal"
+  | SLTerm.star _ l r => do
+    match l with
+    | SLTerm.unrecognized expr =>
+      if (←isDefEq expr rhs) then
+        let impl ← goal.apply' (←mkConstWithFreshMVarLevels ``SLP.entails_self)
+        pure $ SLGoals.mk [] [] impl
+      else
+        let hent :: impl ← goal.apply' (←mkConstWithFreshMVarLevels ``Internal.skip_impure_evidence) | throwError "unexpect goals in skip_impure_evidence"
+        let goals ← solveExactStarMV hent r rhs
+        pure $ goals ++ SLGoals.mk [] [] impl
+    | SLTerm.lift _ => do
+      let hEnt :: impl ← goal.apply' (←mkConstWithFreshMVarLevels ``Internal.skip_pure_evidence) | throwError "unexpect goals in skip_pure_evidence"
+      let (_, hEnt) ← hEnt.intro1
+      let goals ← solveExactStarMV hEnt r rhs
+      pure $ goals ++ SLGoals.mk [] [] impl
+    | _ => do
+      let hEnt :: impl ← goal.apply' (←mkConstWithFreshMVarLevels ``Internal.skip_impure_evidence) | throwError "unexpect goals in skip_impure_evidence"
+      let goals ← solveExactStarMV hEnt r rhs
+      pure $ goals ++ SLGoals.mk [] [] impl
+  | _ => throwError "Unrecognized shape in solveExactStarMV"
 
 mutual
 
@@ -359,84 +297,92 @@ Solves goals of the form `P ⊢ Q ⋆ ?_`, trying to copy as much evidence as po
 -/
 partial def solveStarMV (goal : MVarId) (lhs : SLTerm) (rhsNonMv : SLTerm): TacticM SLGoals := withTraceNode `Lampe.SL (fun e => return f!"solveStarMV {Lean.exceptEmoji e}") do
   match rhsNonMv with
-  | .singleton v _ => solveSingletonStarMV goal lhs v
-  | .lmbSingleton v _ => solveSingletonStarMV goal lhs v
+  | .singleton _ v _ => solveSingletonStarMV goal lhs v
+  | .lmbSingleton _ v _ => solveSingletonStarMV goal lhs v
   | .lift _ => solvePureStarMV goal lhs
-  | .exi _ =>
+  | .exi _ _ =>
     -- solve_exi_prop_star_mv
     let ent₁ :: ent₂ :: impls ← goal.apply' (←mkConstWithFreshMVarLevels ``Internal.solve_exi_prop_star_mv) | throwError "unexpected goals in solve_exi_prop_star_mv"
     let gent₁ ← solveEntailment ent₁
     let (_, ent₂) ← ent₂.intro1
     let gent₂ ← solveEntailment ent₂
-    return gent₁ ++ gent₂ ++ SLGoals.mk [] impls
+    return gent₁ ++ gent₂ ++ SLGoals.mk [] [] impls
+  | .unrecognized expr => solveExactStarMV goal lhs expr
   | _ => throwError "Unrecognized shape in solveStarMV"
 
-partial def solveEntailment (goal : MVarId): TacticM SLGoals := withTraceNode `Lampe.SL (tag := "solveEntailment") (fun e => return f!"solveEntailment {Lean.exceptEmoji e}") do
-  let newGoal ← evalTacticAt (←`(tactic|sl_norm)) goal
-  let goal ← liftOption newGoal[0]?
+partial def solveEntailment (goal : MVarId): TacticM SLGoals := goal.withContext $ withTraceNode `Lampe.SL (tag := "solveEntailment") (fun e => return f!"solveEntailment {Lean.exceptEmoji e}") do
   let target ← goal.instantiateMVarsInType
   let (pre, post) ← parseEntailment target
+  let (pre, preEq) ← Lampe.SL.norm pre
+  let (post, postEq) ← Lampe.SL.norm post
+  let newGoalTp ← mkAppM ``SLP.entails #[pre.expr, post.expr]
+  let nextGoal ← mkFreshMVarId
+  let goalExpr ← mkFreshExprMVarWithId nextGoal (some newGoalTp)
+  let congr ← mkAppM ``Internal.ent_congr #[preEq, postEq, goalExpr]
+  goal.assign congr
+  let goal := nextGoal
 
   trace[Lampe.SL] "Current goal: {pre.printShape} ⊢ {post.printShape}"
   trace[Lampe.SL] (←Lean.PrettyPrinter.ppExpr target)
 
-  match pre with
-  | SLTerm.exi _ => do
-  -- solve_exi_prop_l
-    let g :: impls ← goal.apply' (←mkConstWithFreshMVarLevels ``Internal.solve_exi_prop_l) | throwError "unexpected goals in solve_exi_prop_l"
-    let (_, g) ← g.intro1
-    let newGoals ← solveEntailment g
-    return newGoals ++ SLGoals.mk [] impls
-  | SLTerm.top => do
-    let impls ← goal.apply' (←mkConstWithFreshMVarLevels ``SLP.entails_top)
-    return SLGoals.mk [] impls
-  | SLTerm.lift expr => do
-    if let SLTerm.lift _ := post then
-      return ← solvePureEntailMV goal expr
-  | _ => pure ()
+  goal.withContext do
+    match pre with
+    | SLTerm.exi _ _ => do
+    -- solve_exi_prop_l
+      let g :: impls ← goal.apply' (←mkConstWithFreshMVarLevels ``Internal.solve_exi_prop_l) | throwError "unexpected goals in solve_exi_prop_l"
+      let (_, g) ← g.intro1
+      let newGoals ← solveEntailment g
+      return newGoals ++ SLGoals.mk [] [] impls
+    | SLTerm.top _ => do
+      let impls ← goal.apply' (←mkConstWithFreshMVarLevels ``SLP.entails_top)
+      return SLGoals.mk [] [] impls
+    | SLTerm.lift expr => do
+      if let SLTerm.lift _ := post then
+        return ← solvePureEntailMV goal expr
+    | _ => pure ()
 
-  match post with
-  | SLTerm.mvar _ =>
-    let impls ← goal.apply' (←mkConstWithFreshMVarLevels ``SLP.entails_self)
-    return SLGoals.mk [] impls
-  | SLTerm.top =>
-    let impls ← goal.apply' (←mkConstWithFreshMVarLevels ``SLP.entails_top)
-    return SLGoals.mk [] impls
-  | SLTerm.star _ l r =>
-    -- [TODO] left can be mvar – should be rotated back
-    if r.isMVar then
-      let newGoals ← solveStarMV goal pre l
-      return newGoals
-    else if r.isTop then
-      let g :: impls ← goal.apply' (←mkConstWithFreshMVarLevels ``Internal.star_top_of_star_mvar) | throwError "unexpected goals in star_top_of_star_mvar"
-      let ng ← solveEntailment g
-      return ng ++ SLGoals.mk [] impls
-    else
-      let g₁ :: g₂ :: impls ← goal.apply' (←mkConstWithFreshMVarLevels ``Internal.solve_compose) | throwError "unexpected goals in solve_compose"
-      let ng₁ ← solveEntailment g₁
-      let ng₂ ← solveEntailment g₂
-      return ng₁ ++ ng₂ ++ SLGoals.mk [] impls
-  | SLTerm.singleton _ _ =>
-    -- [TODO] handle pure on the left
-    let impls ← goal.apply' (←mkConstWithFreshMVarLevels ``SLP.entails_self)
-    return SLGoals.mk [] impls
-  | SLTerm.all _ => do
-    let new ← goal.apply' (←mkConstWithFreshMVarLevels ``SLP.forall_right)
-    let new' ← liftOption new[0]?
-    let (_, g) ← new'.intro1
-    solveEntailment g
-  | SLTerm.wand _ _ =>
-    let new ← goal.apply' (←mkConstWithFreshMVarLevels ``SLP.wand_intro)
-    let new' ← liftOption new[0]?
-    solveEntailment new'
-  | SLTerm.exi _ =>
-    -- [TODO] this only works for prop existential - make the others an error
-    let ent₁ :: ent₂ :: impls ← goal.apply' (←mkConstWithFreshMVarLevels ``Internal.solve_exi_prop) | throwError "unexpected goals in solve_exi_prop"
-    let gent₁ ← solveEntailment ent₁
-    let (_, ent₂) ← ent₂.intro1
-    let gent₂ ← solveEntailment ent₂
-    return gent₁ ++ gent₂ ++ SLGoals.mk [] impls
-  | _ => throwError "unknown rhs {post}"
+    match post with
+    | SLTerm.mvar _ =>
+      let impls ← goal.apply' (←mkConstWithFreshMVarLevels ``SLP.entails_self)
+      return SLGoals.mk [] [] impls
+    | SLTerm.top _ =>
+      let impls ← goal.apply' (←mkConstWithFreshMVarLevels ``SLP.entails_top)
+      return SLGoals.mk [] [] impls
+    | SLTerm.star _ l r =>
+      -- [TODO] left can be mvar – should be rotated back
+      if r.isMVar then
+        let newGoals ← solveStarMV goal pre l
+        return newGoals
+      else if r.isTop then
+        let g :: impls ← goal.apply' (←mkConstWithFreshMVarLevels ``Internal.star_top_of_star_mvar) | throwError "unexpected goals in star_top_of_star_mvar"
+        let ng ← solveEntailment g
+        return ng ++ SLGoals.mk [] [] impls
+      else
+        let g₁ :: g₂ :: impls ← goal.apply' (←mkConstWithFreshMVarLevels ``Internal.solve_compose) | throwError "unexpected goals in solve_compose"
+        let ng₁ ← solveEntailment g₁
+        let ng₂ ← solveEntailment g₂
+        return ng₁ ++ ng₂ ++ SLGoals.mk [] [] impls
+    | SLTerm.singleton _ _ _ =>
+      -- [TODO] handle pure on the left
+      let impls ← goal.apply' (←mkConstWithFreshMVarLevels ``SLP.entails_self)
+      return SLGoals.mk [] [] impls
+    | SLTerm.all _ _ => do
+      let new ← goal.apply' (←mkConstWithFreshMVarLevels ``SLP.forall_right)
+      let new' ← liftOption new[0]?
+      let (_, g) ← new'.intro1
+      solveEntailment g
+    | SLTerm.wand _ _ _ =>
+      let new ← goal.apply' (←mkConstWithFreshMVarLevels ``SLP.wand_intro)
+      let new' ← liftOption new[0]?
+      solveEntailment new'
+    | SLTerm.exi _ _ =>
+      -- [TODO] this only works for prop existential - make the others an error
+      let ent₁ :: ent₂ :: impls ← goal.apply' (←mkConstWithFreshMVarLevels ``Internal.solve_exi_prop) | throwError "unexpected goals in solve_exi_prop"
+      let gent₁ ← solveEntailment ent₁
+      let (_, ent₂) ← ent₂.intro1
+      let gent₂ ← solveEntailment ent₂
+      return gent₁ ++ gent₂ ++ SLGoals.mk [] [] impls
+    | _ => throwError "unknown rhs {post}"
 
 end
 
@@ -445,3 +391,11 @@ elab "sl" : tactic => do
   let target ← getMainGoal
   let newGoals ← solveEntailment target
   replaceMainGoal newGoals.flatten
+
+
+-- set_option trace.Lampe.SL true
+
+example : (⟦⟧ : SLP (State p)) ⊢ ⟦⟧ := by
+  apply SLP.entails_trans
+  sl
+  sl
