Lampe/Lampe/Tactic/SL/Term.lean
@@ -1,0 +1,211 @@
+import Lampe.SeparationLogic.State
+import Lampe.SeparationLogic.SLP
+import Lampe.Tactic.SLNorm
+import Lampe.Syntax
+
+import Lean.Meta.Tactic.Simp.Main
+
+open Lean Elab.Tactic Parser.Tactic Lean.Meta Qq
+
+namespace Lampe.SL
+
+inductive SLTerm where
+| top : Lean.Expr → SLTerm
+| star : Lean.Expr → SLTerm → SLTerm → SLTerm
+| lift : Lean.Expr → SLTerm
+| singleton : Lean.Expr → Lean.Expr → Lean.Expr → SLTerm
+| lmbSingleton : Lean.Expr → Lean.Expr → Lean.Expr → SLTerm
+| mvar : Lean.Expr → SLTerm
+| all : Lean.Expr → Lean.Expr → SLTerm
+| exi : Lean.Expr → Lean.Expr → SLTerm
+| wand : Lean.Expr → SLTerm → SLTerm → SLTerm
+| unrecognized : Lean.Expr → SLTerm
+
+def SLTerm.toString : SLTerm → String
+| top _ => "⊤"
+| wand _ a b => s!"{a.toString} -⋆ {b.toString}"
+| exi _ e => s!"∃∃ {e}"
+| all _ e => s!"∀∀ {e}"
+| star _ a b => s!"({a.toString} ⋆ {b.toString})"
+| lift e => s!"{e.dbgToString}"
+| singleton _ e₁ _ => s!"[{e₁.dbgToString} ↦ _]"
+| lmbSingleton _ e₁ _ => s!"[λ {e₁.dbgToString} ↦ _]"
+| mvar e => s!"MV{e.dbgToString}"
+| unrecognized e => s!"<unrecognized: {e.dbgToString}>"
+
+def SLTerm.printShape : SLTerm → String
+| SLTerm.top _ => "⊤"
+| wand _ a b => s!"({a.printShape} -⋆ {b.printShape})"
+| exi _ _ => s!"(∃∃)"
+| all _ _ => s!"(∀∀)"
+| star _ a b => s!"({a.printShape} ⋆ {b.printShape})"
+| lift _ => s!"⟦⟧"
+| singleton _ _ _ => s!"[_ ↦ _]"
+| lmbSingleton _ _ _ => s!"[λ _ ↦ _]"
+| mvar _ => s!"MV"
+| unrecognized _ => s!"<unrecognized>"
+
+def SLTerm.expr : SLTerm → Lean.Expr
+| SLTerm.top e => e
+| SLTerm.star e _ _ => e
+| SLTerm.lift e => e
+| SLTerm.singleton e _ _ => e
+| SLTerm.lmbSingleton e _ _ => e
+| SLTerm.mvar e => e
+| SLTerm.unrecognized e => e
+| SLTerm.wand e _ _ => e
+| SLTerm.exi e _ => e
+| SLTerm.all e _ => e
+
+def SLTerm.isMVar : SLTerm → Bool
+| SLTerm.mvar _ => true
+| _ => false
+
+def SLTerm.isTop : SLTerm → Bool
+| SLTerm.top _ => true
+| _ => false
+
+def SLTerm.isForAll : SLTerm → Bool
+| SLTerm.all _ _ => true
+| _ => false
+
+instance : ToString SLTerm := ⟨SLTerm.toString⟩
+
+instance : Inhabited SLTerm := ⟨SLTerm.top (panic! "empty top")⟩
+
+partial def parseSLExpr (e: Lean.Expr): TacticM SLTerm := do
+  if e.isAppOf' ``SLP.star then
+    let args := e.getAppArgs'
+    let fst ← parseSLExpr (←liftOption args[2]?)
+    let snd ← parseSLExpr (←liftOption args[3]?)
+    return SLTerm.star e fst snd
+  if e.isAppOf' ``State.valSingleton then
+    let args := e.getAppArgs'
+    let fst ← liftOption args[1]?
+    let snd ← liftOption args[2]?
+    return SLTerm.singleton e fst snd
+  else if e.isAppOf' ``State.lmbSingleton then
+    let args := e.getAppArgs'
+    let fst ← liftOption args[1]?
+    let snd ← liftOption args[2]?
+    return SLTerm.lmbSingleton e fst snd
+  else if e.isAppOf' ``SLP.top then
+    return SLTerm.top e
+  else if e.isAppOf' ``SLP.lift then
+    return SLTerm.lift e
+  else if e.getAppFn'.isMVar then
+    return SLTerm.mvar e
+  else if e.isAppOf' ``SLP.forall' then
+    let args := e.getAppArgs'
+    return SLTerm.all e (←liftOption args[3]?)
+  else if e.isAppOf' ``SLP.exists' then
+    let args := e.getAppArgs'
+    return SLTerm.exi e (←liftOption args[3]?)
+  else if e.isAppOf' ``SLP.wand then
+    let args := e.getAppArgs'
+    let lhs ← parseSLExpr (←liftOption args[2]?)
+    let rhs ← parseSLExpr (←liftOption args[3]?)
+    return SLTerm.wand e lhs rhs
+  else pure $ .unrecognized e
+
+partial def parseEntailment (e: Lean.Expr): TacticM (SLTerm × SLTerm) := do
+  if e.isAppOf' ``SLP.entails then
+    let args := e.getAppArgs'
+    let pre ← parseSLExpr (←liftOption args[2]?)
+    let post ← parseSLExpr (←liftOption args[3]?)
+    return (pre, post)
+  else throwError "not an entailment {e}"
+
+partial def solvesSingleton (lhs : SLTerm) (rhsV : Lean.Expr): TacticM Bool :=
+  match lhs with
+  | SLTerm.singleton _ v _ => pure $ v == rhsV
+  | SLTerm.exi _ (Lean.Expr.lam _ _ body _) => do solvesSingleton (←parseSLExpr body) rhsV
+  | _ => pure false
+
+theorem do_star_assoc {p} (a b c : SLP (State p)) : ((a ⋆ b) ⋆ c) = (a ⋆ (b ⋆ c)) := by
+  rw [SLP.star_assoc]
+
+theorem congr_star_r {p} (a b c : SLP (State p)) (eq : b = c) : (a ⋆ b) = (a ⋆ c) := by
+  cases eq
+  rfl
+
+theorem do_star_comm {p} (a b : SLP (State p)) : (a ⋆ b) = (b ⋆ a) := by
+  rw [SLP.star_comm]
+
+theorem do_star_swap {p} (a b c : SLP (State p)) : (a ⋆ b ⋆ c) = (b ⋆ a ⋆ c) := by
+  rw [←SLP.star_assoc]
+  conv => lhs; arg 1; rw [SLP.star_comm]
+  rw [SLP.star_assoc]
+
+partial def linearize (term : SLTerm): TacticM (SLTerm × Lean.Expr) := do
+  match term with
+  | SLTerm.star _ (SLTerm.star _ l r) rr =>
+    let eq ← mkAppM ``do_star_assoc #[l.expr, r.expr, rr.expr]
+    let inner ← mkAppM ``SLP.star #[r.expr, rr.expr]
+    let outer ← mkAppM ``SLP.star #[l.expr, inner]
+    let newTerm := SLTerm.star outer l (SLTerm.star inner r rr)
+    return (newTerm, eq)
+  | SLTerm.star _ l r =>
+    let (r_norm, r_norm_eq) ← linearize r
+    let newExpr ← mkAppM ``SLP.star #[l.expr, r_norm.expr]
+    let eq ← mkAppM ``congr_star_r #[l.expr, r.expr, r_norm.expr, r_norm_eq]
+    return (SLTerm.star newExpr l r_norm, eq)
+  | other => do
+    let eq ← mkAppM ``Eq.refl #[other.expr]
+    return (other, eq)
+
+partial def needs_swap (l r : SLTerm): TacticM Bool := do
+  match l, r with
+  | SLTerm.lift _, SLTerm.lift _ => return false
+  | _, SLTerm.lift _ => return true
+  | _, _ => return false
+
+partial def insert (term : SLTerm): TacticM (SLTerm × Lean.Expr) := do
+  match term with
+  | SLTerm.star e l (SLTerm.star _ ll r) =>
+    if ←needs_swap l ll then
+      let swapEq ← mkAppM ``do_star_swap #[l.expr, ll.expr, r.expr] -- l ⋆ ll ⋆ r = ll ⋆ l ⋆ r
+      let swappedRExpr ← mkAppM ``SLP.star #[l.expr, r.expr]
+      let (insertedR, insertedREq) ← insert (SLTerm.star swappedRExpr l r) -- l ⋆ r = inserted(l ⋆ r)
+      let finalExpr ← mkAppM ``SLP.star #[ll.expr, insertedR.expr]
+      let insertedEq ← mkAppM ``congr_star_r #[ll.expr, swappedRExpr, insertedR.expr, insertedREq] -- ll ⋆ l ⋆ r = ll ⋆ inserted(l ⋆ r)
+      let totalEq ← mkAppM ``Eq.trans #[swapEq, insertedEq]
+      return (SLTerm.star finalExpr l insertedR, totalEq)
+    else
+      let eq ← mkAppM ``Eq.refl #[e]
+      return (term, eq)
+  | SLTerm.star _ l r =>
+    if ←needs_swap l r then
+      let swapEq ← mkAppM ``do_star_comm #[l.expr, r.expr]
+      let swappedExpr ← mkAppM ``SLP.star #[r.expr, l.expr]
+      return (SLTerm.star swappedExpr r l, swapEq)
+    else
+      let eq ← mkAppM ``Eq.refl #[term.expr]
+      return (term, eq)
+  | _ => throwError "shouldn't get here"
+
+partial def sort (term : SLTerm): TacticM (SLTerm × Lean.Expr) := do
+  match term with
+  | SLTerm.star _ l r =>
+    let (r_sorted, r_sorted_eq) ← sort r
+    let newExpr ← mkAppM ``SLP.star #[l.expr, r_sorted.expr]
+    let eq ← mkAppM ``congr_star_r #[l.expr, r.expr, r_sorted.expr, r_sorted_eq]
+    let newTerm := SLTerm.star newExpr l r_sorted
+    let (inserted, inserted_eq) ← insert newTerm
+    let eq ← mkAppM ``Eq.trans #[eq, inserted_eq]
+    return (inserted, eq)
+  | other => do
+    let eq ← mkAppM ``Eq.refl #[other.expr]
+    return (other, eq)
+
+partial def norm (term : SLTerm): TacticM (SLTerm × Lean.Expr) := do
+  let simpResult ← simpOnlyNames [``SLP.star_true, ``SLP.true_star, ``SLP.exists_star, ``SLP.star_exists, ``SLP.exists_pure] term.expr
+  let simped ← parseSLExpr simpResult.expr
+  let (lin, linEq) ← linearize simped
+  let eq ← match simpResult.proof? with
+  | some proof => mkAppM ``Eq.trans #[proof, linEq]
+  | none => pure linEq
+  let (sorted, sortedEq) ← sort lin
+  return (sorted, ←mkAppM ``Eq.trans #[eq, sortedEq])
+
+end Lampe.SL
