stdlib/lampe/Stdlib/Slice.lean
@@ -1,0 +1,61 @@
+import «std-1.0.0-beta.11».Extracted
+import Lampe
+
+open Lampe
+
+open «std-1.0.0-beta.11».Extracted
+
+set_option maxRecDepth 10000
+
+-- TODO: array len needs fixing for this!
+axiom slice_arrayLen {tp: Tp} {p slice} :
+    STHoare p env ⟦⟧ (Expr.callBuiltin [tp.slice] (.u 32) Builtin.arrayLen h![slice]) (fun v => v.toNat = slice.length)
+
+set_option trace.Lampe.STHoare.Helpers true
+set_option trace.Lampe.SL true
+
+lemma for_each_inv {T Env p f fb l}
+    (Inv: List (Tp.denote p T) → SLP (State p))
+    (h_inv: ∀(lp: List (Tp.denote p T)) (e: T.denote p), ((lp ++ [e]) <+: l) → STHoare p env (Inv lp) (fb h![e]) (fun _ => Inv (lp ++ [e]))):
+    STHoare p env (Inv [] ⋆ [λf ↦ fb]) ((«std::slice::for_each».call h![T, Env] h![l, f])) (fun _ => Inv l ⋆ [λf ↦ fb]) := by
+  enter_decl
+  steps []
+  apply STHoare.letIn_intro (Q := fun _ => Inv l ⋆ [λf ↦ fb])
+  · apply STHoare.ramified_frame_top
+      (STHoare.loop_inv_intro' (Inv := fun i _ _ => Inv (l.take i) ⋆ [λf ↦ fb]) ?_)
+    · simp_all
+      simp [Nat.mod_eq_of_lt (by assumption)]
+      sl
+      simp
+    · intro i ihl ihg
+      steps
+      simp_all
+      casesm ∃_,_
+      have : i % 4294967296 = i := by
+        apply Nat.mod_eq_of_lt
+        apply lt_trans ihg
+        apply Nat.mod_lt
+        simp
+      apply STHoare.letIn_intro
+      · apply STHoare.callLambda_intro
+        apply h_inv (lp := l.take i)
+        simp_all [List.take_prefix]
+      · intro
+        steps allow_sl
+        simp_all
+        sl
+  intro
+  steps
+
+lemma slice_map_inv {T U Env p f fb l}
+    (Inv: List (Tp.denote p T) → List (Tp.denote p U) → SLP (State p))
+    (h_inv: ∀(ip: List (Tp.denote p T)) (rp: List (Tp.denote p U)) (e: T.denote p), ((ip ++ [e]) <+: l) → STHoare p env (Inv ip rp) (fb h![e]) (fun r => Inv (ip ++ [e]) (rp ++ [r]))):
+    STHoare p env (Inv [] [] ⋆ [λf ↦ fb]) ((«std::slice::map».call h![T, U, Env] h![l, f])) (fun v => Inv l v ⋆ [λf ↦ fb]) := by sorry
+
+lemma slice_pure_map {T U Env p f fb func l}
+    (h_pure : ∀x, STHoare p env ⟦⟧ (fb h![x]) (fun r => r = func x)):
+    STHoare p env [λf ↦ fb] ((«std::slice::map».call h![T, U, Env] h![l, f])) (fun v => v = l.map func) := by
+  steps [slice_map_inv (Inv := fun i o => o = i.map func)]
+  · rfl
+  · assumption
+  · intros; steps [h_pure]; simp_all
